src/lowparse/LowParse.Spec.Defaultable.fst
@@ -1,0 +1,169 @@
+module LowParse.Spec.Defaultable
+include LowParse.Spec.Base
+include LowParse.Spec.Combinators
+
+module Seq = FStar.Seq
+
+let parse_defaultable_bare (#k: parser_kind) (#t : Type) (defaultablev : option t) (p: parser k t) : Tot (bare_parser t) =
+  fun (input : bytes) ->
+    match defaultablev with
+    | None -> parse p input
+    | Some v -> if (Seq.length input = 0) then Some (v, 0) else (parse p input)
+
+let parse_defaultable_bare_injective (#k : parser_kind) (#t : Type) (defaultablev : option t) (p : parser k t) (b1 b2 : bytes) : Lemma
+  (requires ((parse_defaultable_injective_cond_prop defaultablev p) /\ (injective_precond (parse_defaultable_bare defaultablev p) b1 b2)))
+  (ensures (injective_postcond (parse_defaultable_bare defaultablev p) b1 b2))
+= parser_kind_prop_equiv k p;
+  match defaultablev with
+  | None -> assert (injective_precond p b1 b2)
+  | Some v -> match (Seq.length b1 = 0), (Seq.length b2 = 0) with
+             | true, true -> ()
+             | true, false -> assert (parse_defaultable_injective_cond defaultablev p b2)
+             | false, true -> assert (parse_defaultable_injective_cond defaultablev p b1)
+             | false, false -> assert (injective_precond p b1 b2)
+
+let parse_defaultable (#k: parser_kind) (#t : Type) (defaultablev : option t) (p : parser k t) : Pure (parser (parse_defaultable_kind k) t) 
+  (requires (parse_defaultable_injective_cond_prop defaultablev p))
+  (ensures (fun _ -> True))
+= Classical.forall_intro_2 (fun x -> Classical.move_requires (parse_defaultable_bare_injective defaultablev p x));  
+  parser_kind_prop_equiv k p;
+  parser_kind_prop_equiv (parse_defaultable_kind k) (parse_defaultable_bare defaultablev p);
+  parse_defaultable_bare defaultablev p
+
+let and_then_defaultable'
+  (#k : parser_kind)
+  (#t : eqtype)
+  (p : parser k t)
+  (#k' : parser_kind)
+  (#t' : Type)
+  (fp : t -> parser k' t')
+  (defv : option t')
+  (input : bytes)
+: Lemma
+  (requires (and_then_cases_injective fp /\ (forall (v : t). parse_defaultable_injective_cond_prop defv (fp v))))
+  (ensures (parse_defaultable_injective_cond defv (p `and_then` fp) input))
+= match defv with
+  | None -> ()
+  | Some dv -> 
+    let _ = and_then_eq p fp input in
+    match parse p input with
+    | Some (id, l) -> 
+	let input' = Seq.slice input l (Seq.length input) in
+        assert (parse_defaultable_injective_cond defv (fp id) input')
+    | None -> ()
+
+let and_then_defaultable
+  (#k : parser_kind)
+  (#t : eqtype)
+  (p : parser k t)
+  (#k' : parser_kind)
+  (#t' : Type)
+  (fp : t -> parser k' t')
+  (defv : option t')
+: Lemma
+  (requires (and_then_cases_injective fp /\ (forall (v : t). parse_defaultable_injective_cond_prop defv (fp v))))
+  (ensures (parse_defaultable_injective_cond_prop defv (p `and_then` fp)))
+= Classical.forall_intro (Classical.move_requires (and_then_defaultable' p fp defv))
+
+let nondep_then_defaultable'
+  (#k : parser_kind)
+  (#t : Type)
+  (p : parser k t)
+  (defv : option t)
+  (#k' : parser_kind)
+  (#t' : Type)
+  (p' : parser k' t')
+  (defv' : option t')
+  (input : bytes)
+: Lemma
+  (requires (parse_defaultable_injective_cond_prop defv p))
+  (ensures (parse_defaultable_injective_cond (mk_option_tuple defv defv') (p `nondep_then` p') input))
+= match defv, defv' with
+  | None, _ -> ()
+  | _, None -> ()
+  | Some dv, Some dv' -> 
+    let _ = nondep_then_eq p p' input in
+    match parse p input with
+    | Some (v, l) ->
+        assert (~ (v == dv));
+	(let input' = Seq.slice input l (Seq.length input) in
+        match parse p' input' with
+        | Some (v', l') ->
+          assert (~ ((v, v') == (dv, dv')))
+        | None -> ())
+    | None -> ()
+
+let nondep_then_defaultable
+  (#k : parser_kind)
+  (#t : Type)
+  (p : parser k t)
+  (defv : option t)
+  (#k' : parser_kind)
+  (#t' : Type)
+  (p' : parser k' t')
+  (defv' : option t')
+: Lemma
+  (requires (parse_defaultable_injective_cond_prop defv p))
+  (ensures (parse_defaultable_injective_cond_prop (mk_option_tuple defv defv') (p `nondep_then` p')))
+= Classical.forall_intro (Classical.move_requires (nondep_then_defaultable' p defv p' defv'))
+
+let nondep_then_defaultable_snd'
+  (#k : parser_kind)
+  (#t : Type)
+  (p : parser k t)
+  (defv : option t)
+  (#k' : parser_kind)
+  (#t' : Type)
+  (p' : parser k' t')
+  (defv' : option t')
+  (input : bytes)
+: Lemma
+  (requires (parse_defaultable_injective_cond_prop defv' p'))
+  (ensures (parse_defaultable_injective_cond (mk_option_tuple defv defv') (p `nondep_then` p') input))
+= match defv, defv' with
+  | None, _ -> ()
+  | _, None -> ()
+  | Some dv, Some dv' -> 
+    let _ = nondep_then_eq p p' input in
+    match parse p input with
+    | Some (v, l) ->
+	(let input' = Seq.slice input l (Seq.length input) in
+        match parse p' input' with
+        | Some (v', l') ->
+          assert (~ ((v, v') == (dv, dv')))
+        | None -> ())
+    | None -> ()
+
+let nondep_then_defaultable_snd
+  (#k : parser_kind)
+  (#t : Type)
+  (p : parser k t)
+  (defv : option t)
+  (#k' : parser_kind)
+  (#t' : Type)
+  (p' : parser k' t')
+  (defv' : option t')
+: Lemma
+  (requires (parse_defaultable_injective_cond_prop defv' p'))
+  (ensures (parse_defaultable_injective_cond_prop (mk_option_tuple defv defv') (p `nondep_then` p')))
+= Classical.forall_intro (Classical.move_requires (nondep_then_defaultable_snd' p defv p' defv'))
+
+let defaultable_trivial_eq
+  (#k : parser_kind)
+  (#t : Type)
+  (p : parser k t)
+: Lemma
+  (ensures (forall input. parse (parse_defaultable None p) input == parse p input))
+= ()
+
+let eq_defaultable
+  (#k : parser_kind)
+  (#t : Type)
+  (p : parser k t)
+  (defv : option t)
+  (#k' : parser_kind)
+  (p' : parser k' t)
+: Lemma
+  (requires (parse_defaultable_injective_cond_prop defv p) /\ (forall input. parse p input == parse p' input))
+  (ensures (parse_defaultable_injective_cond_prop defv p'))
+= ()
